theories/Core/Syntactic/CoreInversions.v
@@ -5,7 +5,7 @@ From McPTS.Core.Syntactic Require Export CtxEq.
 Import Syntax_Notations.
 
 
-Lemma wf_pi_inversion {P : PtsSig} : forall {Γ : ctx P} {A B C s1 s2 s3} {r : Ru P s1 s2 s3},
+Lemma wf_pi_inversion {P : PtsSig} : forall {Γ : ctx P} {A B C s1 s2 s3} {r : Ru_pi P s1 s2 s3},
     {{ Γ ⊢ Π r A B : C }} ->
     {{ Γ ⊢ A : Sort@s1 }} /\ {{ Γ, A@s1 ⊢ B : Sort@s2 }} /\ {{ Γ ⊢ Sort@s3 ⊆ C }}.
 Proof with mautosolve 4.
@@ -23,7 +23,7 @@ Qed.
 #[export]
 Hint Resolve wf_pi_inversion : mcpts.
 
-Corollary wf_pi_inversion' {P : PtsSig} : forall {Γ : ctx P} {A B C s1 s2 s3} {r : Ru P s1 s2 s3},
+Corollary wf_pi_inversion' {P : PtsSig} : forall {Γ : ctx P} {A B C s1 s2 s3} {r : Ru_pi P s1 s2 s3},
     {{ Γ ⊢ Π r A B : C }} ->
     {{ Γ ⊢ A : Sort@s1 }} /\ {{ Γ, A@s1 ⊢ B : Sort@s2 }}.
 Proof with mautosolve 4.
@@ -31,7 +31,7 @@ Proof with mautosolve 4.
   destruct_conjs; mauto 2.
 Qed.
 
-Corollary wf_pi_inversion_typ {P} : forall {Γ : ctx P} {A B C s1 s2 s3} {r : Ru P s1 s2 s3},
+Corollary wf_pi_inversion_typ {P} : forall {Γ : ctx P} {A B C s1 s2 s3} {r : Ru_pi P s1 s2 s3},
     {{ Γ ⊢ Π r A B : C }} ->
     {{ Γ ⊢ Sort@s3 ⊆ C }}.
 Proof.
@@ -42,7 +42,7 @@ Qed.
 #[export]
 Hint Resolve wf_pi_inversion' wf_pi_inversion_typ : mcpts.
 
-Corollary wf_typ_pi_inversion {P : PtsSig} : forall {Γ : ctx P} {A B s1 s2 s3} {r : Ru P s1 s2 s3},
+Corollary wf_typ_pi_inversion {P : PtsSig} : forall {Γ : ctx P} {A B s1 s2 s3} {r : Ru_pi P s1 s2 s3},
     {{ Γ ⊢ Π r A B }} ->
     {{ Γ ⊢ A : Sort@s1 }} /\ {{ Γ, A@s1 ⊢ B : Sort@s2 }}.
 Proof.
@@ -52,7 +52,7 @@ Qed.
 #[export]
 Hint Resolve wf_typ_pi_inversion : mcpts.
 
-Corollary wf_typ_pi_inversion' {P : PtsSig} : forall {Γ : ctx P} {A B s1 s2 s3} {r : Ru P s1 s2 s3},
+Corollary wf_typ_pi_inversion' {P : PtsSig} : forall {Γ : ctx P} {A B s1 s2 s3} {r : Ru_pi P s1 s2 s3},
     {{ Γ ⊢ Π r A B }} ->
     {{ Γ ⊢ Π r A B : Sort@s3 }}.
 Proof.
@@ -66,7 +66,7 @@ Qed.
 Hint Resolve wf_typ_pi_inversion' : mcpts.
 
 
-Corollary wf_fn_inversion {P : PtsSig} : forall {Γ : ctx P} {A M C s1 s2 s3} {r : Ru P s1 s2 s3},
+Corollary wf_fn_inversion {P : PtsSig} : forall {Γ : ctx P} {A M C s1 s2 s3} {r : Ru_pi P s1 s2 s3},
     {{ Γ ⊢ λ r A M : C }} ->
     exists B, {{ Γ, A@s1 ⊢ M : B }} /\ {{ Γ ⊢ Π r A B ⊆ C }}.
 Proof with solve [mauto].
@@ -84,7 +84,7 @@ Hint Resolve wf_fn_inversion : mcpts.
 
 Lemma wf_app_inversion {P : PtsSig} : forall {Γ : ctx P} {M N C},
     {{ Γ ⊢ M N : C }} ->
-    exists A B s1 s2 s3 (r : Ru P s1 s2 s3), {{ Γ ⊢ M : Π r A B }} /\ {{ Γ ⊢ N : A }} /\ {{ Γ ⊢ B[Id,,N] ⊆ C }}.
+    exists A B s1 s2 s3 (r : Ru_pi P s1 s2 s3), {{ Γ ⊢ M : Π r A B }} /\ {{ Γ ⊢ N : A }} /\ {{ Γ ⊢ B[Id,,N] ⊆ C }}.
 Proof with mautosolve 4.
   intros * H.
   dependent induction H;
